examples/wysteria/sinterpreter.fst
@@ -16,6 +16,7 @@ open Semantics
 val step: c:config -> Tot (option config)
 let step c =
   if pre_easpar c then Some (step_aspar_e1 c)
+  else if pre_ebox c then Some (step_box_e1 c)
   else if pre_eunbox c then Some (step_unbox_e c)
   else if pre_emkwire c then Some (step_mkwire_e1 c)
   else if pre_eprojwire c then Some (step_projwire_e1 c)
@@ -30,6 +31,7 @@ let step c =
   else if pre_effi c then Some (step_ffi_e c)
   else if pre_ematch c then Some (step_match_e c)
   else if is_value_ps c && is_sframe c is_F_aspar_ps then Some (step_aspar_e2 c)
+  else if is_value_ps c && is_sframe c is_F_box_ps then Some (step_box_e2 c)
   else if is_value c && is_sframe c is_F_mkwire_ps then Some (step_mkwire_e2 c)
   else if is_value_p c && is_sframe c is_F_projwire_p then Some (step_projwire_e2 c)
   else if is_value c && is_sframe c is_F_concatwire_e1 then Some (step_concatwire_e2 c)
@@ -37,7 +39,7 @@ let step c =
   else if is_value c && is_sframe c is_F_ffi then Some (step_ffi_l c)
   else if is_value c && is_sframe c is_F_match then Some (step_match_red c)
   else if is_value c && is_sframe c is_F_aspar_e then Some (step_aspar_red c)
-  //else if is_value c && is_sframe c is_F_box_e then Some (step_box_red c)
+  else if is_value c && is_sframe c is_F_box_e then Some (step_box_red c)
   else if is_value c && is_sframe c is_F_unbox then Some (step_unbox_red c)
   else if is_value c && is_sframe c is_F_mkwire_e then Some (step_mkwire_red c)
   else if is_value c && is_sframe c is_F_projwire_e then Some (step_projwire_red c)
@@ -49,7 +51,7 @@ let step c =
   else if pre_ffi c = Do then Some (step_ffi c)
   else if pre_match c = Do then Some (step_match c)
   else if not (pre_aspar c = NA) then Some (step_aspar c)
-  //else if pre_box c = Do then Some (step_box c)
+  else if pre_box c = Do then Some (step_box c)
   else if pre_unbox c = Do then Some (step_unbox c)
   else if pre_mkwire c = Do then Some (step_mkwire c)
   else if pre_projwire c = Do then Some (step_projwire c)
@@ -67,6 +69,7 @@ val step_correctness: c:config{is_Some (step c)} -> Tot (sstep c (Some.v (step c
 let step_correctness c =
   let c' = v_of_some (step c) in
   if pre_easpar c then C_aspar_ps c c'
+  else if pre_ebox c then C_box_ps c c'
   else if pre_eunbox c then C_unbox c c'
   else if pre_emkwire c then C_mkwire_e1 c c'
   else if pre_eprojwire c then C_projwire_p c c'
@@ -81,6 +84,7 @@ let step_correctness c =
   else if pre_effi c then C_ffi_e c c'
   else if pre_ematch c then C_match_e c c'
   else if is_value_ps c && is_sframe c is_F_aspar_ps then C_aspar_e c c'
+  else if is_value_ps c && is_sframe c is_F_box_ps then C_box_e c c'
   else if is_value c && is_sframe c is_F_mkwire_ps then C_mkwire_e2 c c'
   else if is_value_p c && is_sframe c is_F_projwire_p then C_projwire_e c c'
   else if is_value c && is_sframe c is_F_concatwire_e1 then C_concatwire_e2 c c'
@@ -88,7 +92,7 @@ let step_correctness c =
   else if is_value c && is_sframe c is_F_ffi then C_ffi_l c c'
   else if is_value c && is_sframe c is_F_match then C_match_red c c'
   else if is_value c && is_sframe c is_F_aspar_e then C_aspar_red c c'
-  //else if is_value c && is_sframe c is_F_box_e then C_box_red c c'
+  else if is_value c && is_sframe c is_F_box_e then C_box_red c c'
   else if is_value c && is_sframe c is_F_unbox then C_unbox_red c c'
   else if is_value c && is_sframe c is_F_mkwire_e then C_mkwire_red c c'
   else if is_value c && is_sframe c is_F_projwire_e then C_projwire_red c c'
@@ -100,7 +104,7 @@ let step_correctness c =
   else if pre_ffi c = Do then C_ffi_beta c c'
   else if pre_match c = Do then C_match_beta c c'
   else if not (pre_aspar c = NA) then C_aspar_beta c c'
-  //else if pre_box c = Do then C_box_beta c c'
+  else if pre_box c = Do then C_box_beta c c'
   else if pre_unbox c = Do then C_unbox_beta c c'
   else if pre_mkwire c = Do then C_mkwire_beta c c'
   else if pre_projwire c = Do then C_projwire_beta c c'
